Start simplifying typed mem and structs by removing abstract types.
Tweak has_go_type to make it more obvious to Coq that there's no
infinite recursion. This elimintates the motivation for step-indexed
has_go_type.

src/new_goose_lang/lib/typed_mem/impl.v
@@ -6,67 +6,111 @@ Reserved Notation "![ t ] e"
 Reserved Notation "e1 <-[ t ] e2"
          (at level 80, format "e1  <-[ t ]  e2").
 
-Inductive go_abstract_type :=
-| cellT
-| unitT
-| prodT (t1 t2 : go_abstract_type)
-.
-Fixpoint go_abstract_type_size (t : go_abstract_type) : nat :=
+Fixpoint go_type_size (t : go_type) : nat :=
   match t with
-  | prodT t1 t2 => go_abstract_type_size t1 + go_abstract_type_size t2
-  | cellT => 1
-  | unitT => 0
+  | structT d =>
+      (fix go_type_size_struct d : nat :=
+        match d with
+        | [] => O
+        | (_,t) :: d => (go_type_size t + go_type_size_struct d)%nat
+        end
+      ) d
+  | sliceT e => 3
+  | interfaceT => 3
+  | _ => 1
   end.
-
-Fixpoint go_type_interp (t : go_type) : go_abstract_type :=
-  match t with
-  | sliceT _ => (prodT (prodT cellT cellT) cellT)
-  | structT decls => fold_right prodT unitT (fmap (go_type_interp ∘ snd) decls)
-  | interfaceT => prodT (prodT cellT cellT) cellT (* type id, val, methods *)
-  | _ => cellT
-  end.
-
-Definition go_type_size (t : go_type) : nat := go_abstract_type_size $ go_type_interp t.
 
 
 Reserved Notation "l +ₗ[ t ] z" (at level 50, left associativity, format "l  +ₗ[ t ]  z").
-Notation "l +ₗ[ t ] z" := (l +ₗ go_abstract_type_size (go_type_interp t) * z) : stdpp_scope .
-Notation "e1 +ₗ[ t ] e2" := (BinOp (OffsetOp (go_abstract_type_size $ go_type_interp t)) e1%E e2%E) : expr_scope .
+Notation "l +ₗ[ t ] z" := (l +ₗ go_type_size t * z) : stdpp_scope .
+Notation "e1 +ₗ[ t ] e2" := (BinOp (OffsetOp (go_type_size t)) e1%E e2%E) : expr_scope .
 
 Section go_lang.
   Context `{ffi_syntax}.
+  Local Coercion Var' (s:string): expr := Var s.
 
   (** allocation with a type annotation *)
   Definition ref_to (t:go_type): val := λ: "v", ref (Var "v").
 
   (* TODO: seal *)
   Definition load_ty (t : go_type) : val :=
-    (fix load_ty_aux t : val :=
-      match t with
-      | prodT t1 t2 => (λ: "l", (load_ty_aux t1 (Var "l"),
-                                  load_ty_aux t2 (BinOp (OffsetOp (go_abstract_type_size t1))
-                                                                  (Var "l") #1)))%V
-      | cellT => (λ: "l", !(Var "l"))%V
-      | unitT => (λ: <>, #())%V
-      end) (go_type_interp t).
+    match t with
+    | structT d =>
+        (fix store_struct d : val :=
+          match d with
+          | [] => (λ: <>, #())%V
+          | (f,t) :: d => (λ: "pv", let: "p" := Fst "pv" in
+                                  let: "v" := Snd "pv" in
+                                  store_ty_aux t ("p", Fst "v");;
+                                  store_struct d (BinOp (OffsetOp (go_type_size t))
+                                                        "p" #1, Snd "v"))%V
+          end) d
+    | sliceT e =>
+        (λ: "pv", let: "p" := Fst "pv" in
+                  let: "v" := Snd "pv" in
+                  let: (("a", "b"), "c") := "v" in
+                  "p" +ₗ #0 <- "a" ;;
+                  "p" +ₗ #1 <- "b" ;;
+                  "p" +ₗ #2 <- "c"
+        )%V
 
-  Definition store_ty t: val :=
-    (fix store_ty_aux t : val :=
-       match t with
-       | prodT t1 t2 => (λ: "pv",
-                         let: "p" := Fst (Var "pv") in
-                         let: "v" := Snd (Var "pv") in
-                         store_ty_aux t1 (Var "p", Fst (Var "v"));;
-                         store_ty_aux t2 (BinOp (OffsetOp (go_abstract_type_size t1))
-                                                          (Var "p") #1, Snd (Var "v")))%V
-       | cellT => (λ: "pv", Fst (Var "pv") <- Snd (Var "pv"))%V
-       | unitT => (λ: <>, #())%V
-       end) (go_type_interp t).
+    | interfaceT =>
+        (λ: "pv", let: "p" := Fst "pv" in
+                  let: "v" := Snd "pv" in
+                  let: (("a", "b"), "c") := "v" in
+                  "p" +ₗ #0 <- "a" ;;
+                  "p" +ₗ #1 <- "b" ;;
+                  "p" +ₗ #2 <- "c"
+        )%V
+
+    | cellT => (λ: "l", !(Var "l"))%V
+    end.
+
+    match t with
+    | prodT t1 t2 => (λ: "l", (load_ty_aux t1 (Var "l"),
+                               load_ty_aux t2 (BinOp (OffsetOp (go_abstract_type_size t1))
+                                                     (Var "l") #1)))%V
+    | cellT => (λ: "l", !(Var "l"))%V
+    | unitT => (λ: <>, #())%V
+    end) (go_type_interp t).
+
+  Fixpoint store_ty (t : go_type): val :=
+    match t with
+    | structT d =>
+        (fix store_struct d : val :=
+          match d with
+          | [] => (λ: <>, #())%V
+          | (f,t) :: d => (λ: "pv", let: "p" := Fst "pv" in
+                                  let: "v" := Snd "pv" in
+                                  store_ty_aux t ("p", Fst "v");;
+                                  store_struct d (BinOp (OffsetOp (go_type_size t))
+                                                        "p" #1, Snd "v"))%V
+          end) d
+    | sliceT e =>
+        (λ: "pv", let: "p" := Fst "pv" in
+                  let: "v" := Snd "pv" in
+                  let: (("a", "b"), "c") := "v" in
+                  "p" +ₗ #0 <- "a" ;;
+                  "p" +ₗ #1 <- "b" ;;
+                  "p" +ₗ #2 <- "c"
+        )%V
+
+    | interfaceT =>
+        (λ: "pv", let: "p" := Fst "pv" in
+                  let: "v" := Snd "pv" in
+                  let: (("a", "b"), "c") := "v" in
+                  "p" +ₗ #0 <- "a" ;;
+                  "p" +ₗ #1 <- "b" ;;
+                  "p" +ₗ #2 <- "c"
+        )%V
+
+    | _ => (λ: "pv", Fst "pv" <- Snd "pv")%V
+    end.
 
   Definition ref_ty (t : go_type) : val := λ: "v", ref (Var "v").
 End go_lang.
 
-Notation "![ t ] e" := (load_ty t e%E) : expr_scope.
+(* otation "![ t ] e" := (load_ty t e%E) : expr_scope. *)
 (* NOTE: in code we want to supply arbitrary expressions, so we have the usual
    notation, but the specs should be in terms of value pairs, so we have a
    similar notation in the value-scope (even though this is an expression and
@@ -74,5 +118,6 @@ Notation "![ t ] e" := (load_ty t e%E) : expr_scope.
 
    See the HeapLang documentation in Iris for par, which has a similar
    trick. *)
+(* FIXME: these notations are a little messed up; they get unfolded where they shouldn't, etc. *)
 Notation "e1 <-[ t ] e2" := (store_ty t (Pair e1%E e2%E)) : expr_scope.
 Notation "v1 <-[ t ] v2" := (store_ty t (PairV v1%V v2%V)) : val_scope.
